$$ δN = δ \int f(\vec{r}) W(\vec{r})^2 d\vec{r} = \int f(\vec{r}) δ(W(\vec{r})^2) d\vec{r} = \int f(\vec{r}) 2 W(\vec{r}) δW(\vec{r}) d\vec{r} $$

$$
δD = δ \int g(\vec{r}) W(\vec{r}) d\vec{r} = \int g(\vec{r}) δW(\vec{r}) d\vec{r}
$$

$$
(\int f(\vec{r}) 2 W(\vec{r}) δW(\vec{r}) d\vec{r}) \cdot (\int g(\vec{r}') W(\vec{r}') d\vec{r}') - 2 (\int f(\vec{r}') W(\vec{r}')^2 d\vec{r}') \cdot (\int g(\vec{r}) δW(\vec{r}) d\vec{r}) = 0
$$

$$
\int \left[ 2 f(\vec{r}) W(\vec{r}) (\int g(\vec{r}') W(\vec{r}') d\vec{r}') - 2 g(\vec{r}) (\int f(\vec{r}') W(\vec{r}')^2 d\vec{r}') \right] δW(\vec{r}) d\vec{r} = 0
$$

$$
2 f(\vec{r}) W(\vec{r}) (\int g(\vec{r}') W(\vec{r}') d\vec{r}') - 2 g(\vec{r}) (\int f(\vec{r}') W(\vec{r}')^2 d\vec{r}') = 0
$$

$$
f(\vec{r}) W(\vec{r}) (\int g(\vec{r}') W(\vec{r}') d\vec{r}') = g(\vec{r}) (\int f(\vec{r}') W(\vec{r}')^2 d\vec{r}')
$$